template-coq/theories/Universes.v
@@ -699,6 +699,8 @@ End Universe.
 Definition is_propositional u := 
   Universe.is_prop u || Universe.is_sprop u.
 
+Definition relevance_of_sort s := if (Universe.is_sprop s) then Relevant else Irrelevant.
+
 (** This coercion allows to see the universes as a [UnivExprSet.t] *)
 Coercion Universe.t_set : Universe.nonEmptyUnivExprSet >-> UnivExprSet.t.
 
